Roos/Dyck_Language.thy
@@ -15,34 +15,37 @@ lemma destTm_Tm[simp]: \<open>destTm \<circ> Tm = id\<close>
 by auto
 (* until here*)
 
-text \<open>Dyck languages are sets of words/lists of balanced brackets.\<close>
+text \<open>Dyck languages are sets of words/lists of balanced brackets. A bracket is a pair of type
+\<^typ>\<open>bool \<times> 'a\<close> where \<open>True\<close> is an opening and \<open>False\<close> a closing bracket. Brackets are tagged with
+elements of type \<open>'a\<close>.\<close>
+
+type_synonym 'a bracket = "bool \<times> 'a"
+
+abbreviation "Open a \<equiv> (True,a)"
+abbreviation "Close a \<equiv> (False,a)"
 
 subsection\<open>Balanced\<close>
 
-text\<open>A type of brackets for creating the \emph{Dyck_lang}\<close>
-datatype bracket = Open | Close
+text\<open>Definition of what it means to be a \emph{balanced} list of brackets:\<close>
 
-text\<open>Definition of what it means to be a \emph{balanced} list with elements of type \<open>bracket \<times> 'a\<close>,
-i.e.\ the brackets are indexed with elements of type \<open>'a\<close>, i.e.\ we have multiple brackets.\<close>
-
-inductive bal :: "(bracket  \<times> 'a) list \<Rightarrow> bool" where
+inductive bal :: "'a bracket list \<Rightarrow> bool" where
   "bal []" |
   "bal xs \<Longrightarrow> bal ys \<Longrightarrow> bal (xs @ ys)" | 
-  "bal xs \<Longrightarrow> bal ((Open, g) # xs @ [(Close, g)])" 
+  "bal xs \<Longrightarrow> bal (Open a # xs @ [Close a])" 
 
 declare bal.intros(1)[iff] bal.intros(2)[intro,simp] bal.intros(3)[intro!,simp]
 
-lemma bal2[iff]: "bal [(Open,g), (Close,g)]" 
+lemma bal2[iff]: "bal [Open a, Close a]" 
   using bal.intros(3) by fastforce
 
 text \<open>The inductive definition of balanced is complemented with a functional version
 that uses a stack to remember which opening brackets need to be closed:\<close>
 
-fun bal_stk :: "'a list \<Rightarrow> (bracket \<times> 'a) list \<Rightarrow> 'a list * (bracket \<times> 'a) list" where
+fun bal_stk :: "'a list \<Rightarrow> 'a bracket list \<Rightarrow> 'a list * 'a bracket list" where
   "bal_stk s [] = (s,[])" |
-  "bal_stk s ((Open, a) # bs) = bal_stk (a # s) bs" |
-  "bal_stk (a' # s) ((Close, a) # bs) =
-    (if a = a' then bal_stk s bs else (a' # s, (Close, a) # bs))" | 
+  "bal_stk s (Open a # bs) = bal_stk (a # s) bs" |
+  "bal_stk (a' # s) (Close a # bs) =
+    (if a = a' then bal_stk s bs else (a' # s, Close a # bs))" | 
   "bal_stk bs stk = (bs,stk)"
 
 lemma bal_stk_append:
@@ -60,7 +63,7 @@ lemma bal_stk_if_bal:  "bal xs \<Longrightarrow> bal_stk s xs = (s,[])"
 by(induction arbitrary: s rule: bal.induct)(auto split: if_splits)
 
 lemma bal_insert_AB:
-  "bal u \<Longrightarrow> u = v@w \<Longrightarrow> bal (v @ (Open, x) # (Close, x) # w)"
+  "bal u \<Longrightarrow> u = v@w \<Longrightarrow> bal (v @ (Open x # Close x # w))"
 proof(induction arbitrary: v w rule: bal.induct)
   case 1 thus ?case by blast
 next
@@ -68,11 +71,11 @@ next
   show ?case
   proof (cases v)
     case Nil
-    hence "w = ((Open, y)) # u @ [(Close, y)]" using "3.prems" 
+    hence "w = (Open y) # u @ [Close y]" using "3.prems" 
       by simp
     hence "bal w" using "3.hyps" 
       by blast
-    hence "bal ([(Open, x), (Close, x)] @ w)" 
+    hence "bal ([Open x, Close x] @ w)" 
       by blast
     thus ?thesis using Nil by simp
   next
@@ -80,13 +83,13 @@ next
     show ?thesis
     proof (cases w rule:rev_cases)
       case Nil
-      from "3.hyps" have "bal (((Open, x) # u @ [(Close, x)]) @ [(Open, x), (Close, x)])"
+      from "3.hyps" have "bal ((Open x # u @ [Close x]) @ [Open x, Close x])"
         using bal.intros(2) by blast
       thus ?thesis using Nil Cons 3
         by (metis append_Nil append_Nil2 bal.simps)
     next
       case (snoc w' Y)
-      hence u: "u=v'@w'" and [simp]: "X=(Open, y) & Y=(Close, y)"
+      hence u: "u=v'@w'" and [simp]: "X= Open y & Y= Close y"
         using Cons "3.prems" apply (smt (verit, ccfv_threshold) List.append.assoc List.list.inject append_Cons append_eq_append_conv last_snoc)
         by (metis "local.3.prems" Cons List.append.assoc List.list.inject append_Cons last_snoc snoc)
           \<comment> \<open>This also works by auto, but it takes 4 seconds.\<close>
@@ -101,22 +104,22 @@ next
   thus ?case
   proof
     assume A: ?A
-    hence "bal (v @ (Open, x) # (Close, x) # r)" 
+    hence "bal (v @ Open x # Close x # r)" 
       using "2.IH"(1) by presburger
-    hence "bal ((v @ (Open, x) # (Close, x)#r) @ w')" 
+    hence "bal ((v @ Open x # Close x#r) @ w')" 
       using \<open>bal w'\<close> by(rule bal.intros(2))
     thus ?thesis using A by auto
   next
     assume B: ?B
-    hence "bal (r @ (Open, x) # (Close, x) # w)" 
+    hence "bal (r @ Open x # Close x # w)" 
       using "2.IH"(2) by presburger
-    with \<open>bal v'\<close> have "bal (v'@(r@(Open, x) # (Close, x)#w))" 
+    with \<open>bal v'\<close> have "bal (v'@(r@Open x # Close x#w))" 
       by(rule bal.intros(2))
     thus ?thesis using B by force
   qed 
 qed 
 
-lemma bal_if_bal_stk: "bal_stk s w = ([],[]) \<Longrightarrow> bal (rev(map (\<lambda>x. (Open, x)) s) @ w)"
+lemma bal_if_bal_stk: "bal_stk s w = ([],[]) \<Longrightarrow> bal (rev(map (\<lambda>x. Open x) s) @ w)"
 proof(induction s w rule: bal_stk.induct)
   case 2
   then show ?case by simp
@@ -199,23 +202,23 @@ corollary bal_iff_insert[iff]:
   shows \<open>bal (v @ b @ w) = bal (v @ w)\<close>
   using bal_del bal_insert by (metis assms)
 
-lemma bal_start_Open: \<open>bal (x#xs) \<Longrightarrow>\<exists>g. x = (Open,g)\<close>
+lemma bal_start_Open: \<open>bal (x#xs) \<Longrightarrow>\<exists>a. x = Open a\<close>
   using bal_stk.elims bal_stk_iff_bal by blast 
 
 lemma bal_Open_split: assumes bal_x_xs: \<open>bal (x # xs)\<close>
-  shows \<open>\<exists>y r g. bal y \<and> bal r \<and> (x # xs) = (Open, g) # y @ (Close, g) # r\<close>
+  shows \<open>\<exists>y r a. bal y \<and> bal r \<and> (x # xs) = Open a # y @ Close a # r\<close>
 proof-
-  from bal_x_xs obtain g where x_def: \<open>x = (Open, g)\<close> 
+  from bal_x_xs obtain a where x_def: \<open>x = Open a\<close> 
     using bal_start_Open by blast
-  then have \<open>bal ((Open, g) # xs) \<Longrightarrow> \<exists>y r. bal y \<and> bal r \<and> (x # xs) = (Open, g) # y @ (Close, g) # r\<close>
+  then have \<open>bal (Open a # xs) \<Longrightarrow> \<exists>y r. bal y \<and> bal r \<and> (x # xs) = Open a # y @ Close a # r\<close>
   proof(induction \<open>length (x # xs)\<close> arbitrary: xs rule: less_induct)
     case less
-    have IH: \<open>\<And>w. \<lbrakk>length ((Open, g) # w) < length ((Open, g) # xs); bal ((Open, g) # w)\<rbrakk> \<Longrightarrow> \<exists>y r. bal y \<and> bal r \<and> (Open, g) # w = (Open, g) # y @ (Close, g) # r\<close> 
+    have IH: \<open>\<And>w. \<lbrakk>length (Open a # w) < length (Open a # xs); bal (Open a # w)\<rbrakk> \<Longrightarrow> \<exists>y r. bal y \<and> bal r \<and> Open a # w = Open a # y @ Close a # r\<close> 
       using less by blast
-    have \<open>bal ((Open, g) # xs)\<close> 
+    have \<open>bal (Open a # xs)\<close> 
       using less bal_x_xs by blast
     then show ?case
-    proof(induction \<open>(Open,g) # xs\<close> rule: bal.induct)
+    proof(induction \<open>Open a # xs\<close> rule: bal.induct)
       case (2 as bs)
       consider (as_empty)  \<open>as = []\<close> | (bs_empty)\<open>bs = []\<close> | (both_not_empty)\<open>as \<noteq> [] \<and> bs \<noteq> []\<close> by blast
       then show ?case
@@ -227,13 +230,13 @@ proof-
         then show ?thesis using 2 by (metis append_self_conv)
       next
         case both_not_empty
-        then obtain as' where as'_def: \<open>(Open, g) # as' = as\<close> 
+        then obtain as' where as'_def: \<open>Open a # as' = as\<close> 
           using 2 by (metis append_eq_Cons_conv)
-        then have \<open>length ((Open, g) # as') < length ((Open, g) # xs)\<close> 
+        then have \<open>length (Open a # as') < length (Open a # xs)\<close> 
           by (metis "local.2.hyps"(5) List.append.right_neutral append_eq_conv_conj both_not_empty linorder_not_le take_all_iff)
-        with IH \<open>bal as\<close> obtain y r where yr_def: \<open>bal y \<and> bal r \<and> (Open, g) # as' = (Open, g) # y @ (Close, g) # r\<close> 
+        with IH \<open>bal as\<close> obtain y r where yr_def: \<open>bal y \<and> bal r \<and> Open a # as' = Open a # y @ Close a # r\<close> 
           using as'_def by meson
-        then have \<open>(Open, g) # xs = (Open, g) # y @ (Close, g) # r @ bs\<close> 
+        then have \<open>Open a # xs = Open a # y @ Close a # r @ bs\<close> 
           using as'_def by (metis "local.2.hyps"(5) List.append.assoc append_Cons)
         moreover have \<open>bal y\<close> and \<open>bal (r@bs)\<close> 
           using yr_def apply blast by (simp add: "local.2.hyps"(3) yr_def)
@@ -256,7 +259,7 @@ abbreviation snds_in :: \<open>'a set  \<Rightarrow> ('b  \<times> 'a) list \<Ri
 
 text\<open>The Dyck/bracket language over a set \<open>\<Gamma>\<close> is the set of balanced words over \<open>\<Gamma>\<close>:\<close>
 
-definition Dyck_lang :: "'a set \<Rightarrow> (bracket  \<times> 'a) list set" where
+definition Dyck_lang :: "'a set \<Rightarrow> 'a bracket list set" where
 "Dyck_lang \<Gamma> = {w. bal w \<and> snds_in \<Gamma> w}"
 
 lemma Dyck_langI[intro]: 
@@ -305,7 +308,7 @@ lemma bal_tm_Nt[iff]:\<open>bal_tm [Nt A]\<close>
 lemma bal_tm_append[intro, simp]: \<open>bal_tm xs \<Longrightarrow> bal_tm ys \<Longrightarrow> bal_tm (xs @ ys)\<close> 
   unfolding bal_tm_def by simp
 
-lemma bal_tm_surr[intro!, simp]: \<open>bal_tm xs \<Longrightarrow> bal_tm (Tm (Open, g) # xs @ [Tm (Close, g)])\<close> 
+lemma bal_tm_surr[intro!, simp]: \<open>bal_tm xs \<Longrightarrow> bal_tm (Tm (Open a) # xs @ [Tm (Close a)])\<close> 
   unfolding bal_tm_def by simp
 
 lemma bal_tm_prepend_Nt[intro!, simp]: \<open>bal_tm xs \<Longrightarrow> bal_tm (Nt A # xs)\<close> 
@@ -314,10 +317,10 @@ lemma bal_tm_prepend_Nt[intro!, simp]: \<open>bal_tm xs \<Longrightarrow> bal_tm
 lemma bal_tm_append_Nt[intro!, simp]: \<open>bal_tm xs \<Longrightarrow> bal_tm (xs@[Nt A])\<close> 
   by blast
 
-lemma bal_tm2[iff]: "bal_tm [Tm (Open,g), Tm (Close,g)]" 
+lemma bal_tm2[iff]: "bal_tm [Tm (Open a), Tm (Close a)]"
   using bal_tm_surr by force
 
-lemma bal_tm2_Nt[iff]: "bal_tm [Tm (Open,g), Tm (Close,g), Nt A]" 
+lemma bal_tm2_Nt[iff]: "bal_tm [Tm (Open a), Tm (Close a), Nt A]" 
   using bal_tm_append_Nt by force
 
 (* TODO: now in CFG *)
@@ -333,22 +336,26 @@ lemma bal_tm_imp_bal_for_tms: \<open>bal_tm (map Tm xs') \<Longrightarrow> bal x
   unfolding bal_tm_def by auto
 
 
-subsection\<open>Function \<^term>\<open>snds_in_tm\<close>\<close>
+subsection\<open>Function \<open>snds_in_tm\<close>\<close>
 
-text\<open>Version of \<^term>\<open>snds_in\<close> but for a list of symbols, that might contain Nonterminals.
+text\<open>Version of \<open>snds_in\<close> but for a list of symbols, that might contain Nonterminals.
 Says that all right hand sides of \<open>x\<close> (here stripped of their \<open>Tm\<close>) are in \<open>\<Gamma>\<close>:\<close>
 definition snds_in_tm where
   \<open>snds_in_tm \<Gamma> \<equiv> snds_in \<Gamma> o map destTm o filter isTm\<close>
-
+(*
 text\<open>Useful lemmas about this:\<close>
 lemma snds_in_tm_del_right: \<open>snds_in_tm \<Gamma> (xs@ys) \<Longrightarrow> snds_in_tm \<Gamma> xs\<close> 
   unfolding snds_in_tm_def by auto
 
 lemma snds_in_tm_del_left: \<open>snds_in_tm \<Gamma> (xs@ys) \<Longrightarrow> snds_in_tm \<Gamma> ys\<close>
   unfolding snds_in_tm_def by auto
+*)
+lemma snds_in_tm_Nt[simp]:
+  \<open>snds_in_tm \<Gamma> (Nt A # xs) = snds_in_tm \<Gamma> xs\<close>
+unfolding snds_in_tm_def by auto
 
 lemma snds_in_tm_append[simp]:
-  \<open>snds_in_tm \<Gamma> xs \<Longrightarrow> snds_in_tm \<Gamma> ys \<Longrightarrow> snds_in_tm \<Gamma> (xs@ys)\<close>
+  \<open>snds_in_tm \<Gamma> (xs@ys) = (snds_in_tm \<Gamma> xs \<and> snds_in_tm \<Gamma> ys)\<close>
 unfolding snds_in_tm_def by auto
 
 text\<open>Relationship between \<^term>\<open>bal_tm\<close>, \<^term>\<open>snds_in_tm\<close> and \<open>Dyck_Language\<close>\<close>
@@ -363,7 +370,7 @@ subsection\<open>Lifting \<^const>\<open>bal\<close> and \<^const>\<open>bal_tm\
 subsubsection\<open>Function \<open>bal_stk_tm\<close>\<close>
 
 text\<open>A version of \<^term>\<open>bal_stk\<close> but for a symbol list that might contain nonterminals (they are ignored via filtering).\<close>
-definition bal_stk_tm :: "'t list \<Rightarrow> ('n, bracket \<times> 't) syms \<Rightarrow> 't list * ('n, bracket \<times> 't) syms" where
+definition bal_stk_tm :: "'t list \<Rightarrow> ('n, 't bracket) syms \<Rightarrow> 't list * ('n, 't bracket) syms" where
 \<open>bal_stk_tm x y \<equiv>
   (fst ((bal_stk x o map destTm o filter isTm) y), map Tm (snd ((bal_stk x o map destTm o filter isTm) y)))\<close>
 
@@ -381,7 +388,7 @@ lemma bal_stk_tm_if_bal_tm: "bal_tm xs \<Longrightarrow> bal_stk_tm s xs = (s,[]
   unfolding bal_stk_tm_def 
   by (simp add: bal_tm_def bal_stk_if_bal)+
 
-lemma bal_tm_insert_AB: assumes u: "bal_tm u" shows "u = v@w \<Longrightarrow> bal_tm (v @ Tm (Open, x) # Tm (Close, x) # w)" using u
+lemma bal_tm_insert_AB: assumes u: "bal_tm u" shows "u = v@w \<Longrightarrow> bal_tm (v @ Tm (Open x) # Tm (Close x) # w)" using u
 unfolding bal_tm_def by (auto intro!: bal_insert_AB)
 
 lemma bal_tm_insert_Nt: "bal_tm u \<Longrightarrow> u = v@w \<Longrightarrow> bal_tm (v @ Nt A # w)"
